\documentclass{article}

\renewcommand{\thesection}{}

\usepackage{amsmath}

\begin{document}

	\section{2.1 Exercises}

	\begin{enumerate}
		% TODO: Q1
		\item
		\begin{enumerate}
			\item Find the slope of the tangent line to the parabola
				$y = 4x - x^2$ at the point $(1,3)$

			\begin{enumerate}
				\item using Definition 1

				\item using Equation 2
			\end{enumerate}

			\item Find an equation of the tangent line in part (a).

			\item Graph an equation of the tangent line in part (a).
		\end{enumerate}

		% TODO: Q2
		\item
		\begin{enumerate}
			\item Find the slope of the tangent line to the curve $y = x^3$ at
				the point $(-1,-1)$.

			\begin{enumerate}
				\item using Definition 1

				\item using Definition 2
			\end{enumerate}

			\item Find an equation of the tangent line in part (a).

			\item Graph the curve and the tangent line in successively smaller
				viewing rectangles centered at $(-1,-1)$ until the curve and
				the line appear to coincide.
		\end{enumerate}

		\item[3-6] Find an equation of the tangent line to the curve at the given point.
		% Q3
		\item $y = 4x - 3x^2, (2, -4)$

			$$\lim \limits _{x \to 2} \frac{4x - 3x^2 - (-4)}{x-2}$$

			$$\lim \limits _{x \to 2} \frac{4x - 3x^2 + 4}{x-2}$$

			$$\lim \limits _{x \to 2} \frac{-(3x^2 - 4x - 4}{x-2}$$

			$$\lim \limits _{x \to 2} \frac{-(3x+2)(x-2)}{x-2}$$

			$$\lim \limits _{x \to 2} -3x-2$$

			$$m = -3(2) - 2 = -8$$

			The equation of the tangent line would be

			$$y - (-4) = -8(x - 2)$$

			$$y + 4 = -8x + 16$$
			
			$$y = -8x - 12$$

		% Q4
		\item $y = 2x^3 - 5x, (-1, 3)$

			$$m = \lim \limits _{h \to 0} \frac{2(-1+h)^3 - 5(-1+h) - (2(-1)^3 - 5(-1))}{h}$$

			$$m = \lim \limits _{h \to 0} \frac{2(-1+h)^3 - 5(-1 + h) - 3}{h}$$

			$$m = \lim \limits _{h \to 0} \frac{2(h^3 - 3h^2 + 3h -1) -3 + 5 - 5h}{h}$$

			$$m = \lim \limits _{h \to 0} \frac{2h^3 - 6h^2 + 6h -2 + 2 - 5h}{h}$$

			$$m = \lim \limits _{h \to 0} \frac{2h^3 - 6h^2 + 6h - 5h}{h}$$

			$$m = \lim \limits _{h \to 0} \frac{2h^3 - 6h^2 + h}{h}$$

			$$m = \lim \limits _{h \to 0} 6h + 1 = 1$$

			So we find the equation by

			$$y - 3 = x - (-1)$$

			$$y - 3 = x + 1$$

			$$y = x + 4$$
		% Q5
		\item $y = \sqrt{x}, (1,1)$

			$$\lim \limits _{x \to a} \frac{f(x) - f(a)}{x - a}$$

			$$\lim \limits _{x \to 1} \frac{\sqrt{x} - 1}{x-1}$$

			$$\frac{\sqrt{x} - 1}{x-1} \times \frac{\sqrt{x} + 1}{\sqrt{x} + 1} = 
				\frac{(\sqrt{x} - 1)(\sqrt{x} + 1)}{(x-1)(\sqrt{x}+1)}$$

			$$(\sqrt{x}-1)(\sqrt{x}+1) = x-1$$

			$$\frac{x-1}{(x-1)(\sqrt{x}+1)} = \frac{1}{\sqrt{x}+1}$$

			$$\lim \limits _{x \to 1} \frac{1}{\frac{x} + 1} = \frac{1}{2}$$

			$$y - 1 = \frac{1}{2}(x-1)$$

			$$y = \frac{1}{2}x + \frac{1}{2}$$

		% Q6
		\item $y = \frac{2x + 1}{x+2}, (1,1)$

			$$m = \lim \limits _{x \to a} \frac{f(x) - f(a)}{x -a}$$

			$$m = \lim \limits _{x \to 1} \frac{(2x+1) - (2(1)+1)}{x-1}$$

			$$m = \lim \limits _{x \to 1} \frac{(2x+1) - 3}{x-1}$$

			$$m = \lim \limits _{x \to 1} \frac{2x-2}{x-1}$$

			$$m = \lim \limits _{x \to 1} \frac{2(x-1)}{x-1} = 2$$

			So the equation is...

			$$y - 1 = 2(x - 1)$$

			$$y - 1 = 2x - 2$$

			$$y = 2x - 1$$

		% TODO Q7
		\item 
			\begin{enumerate}
				\item Find the slope of the tangent to the curve $y = 3 + 4x^2 - 2x^3$
					at the point where $x = a$

				\item Find equations of the tangent lines at the points $(1,5)$ and
					$(2,3)$.

				\item Graph the curve and both tangents on a common screen.
			\end{enumerate}
		% TODO Q8
		\item 
		\begin{enumerate}
			\item Find the slope of the tangent to the curve $y = 1/\sqrt{x}$ at the point
				where $x=a$

			\item Find the equations of the tangent lines at the points $(1,1)$ and $(4, \frac{1}{4})$.

			\item Graph the curve and both tangents on a common screen.
		\end{enumerate}
		% TODO Q9
		\item The graph shows the position function of a car. Use the shape of the graph to explain your
			answers to the following questions.
		\begin{enumerate}
			\item What was the initial velocity of the car?

			\item Was the car going faster at $B$ or $C$?

			\item Was the car slowing down or speeding up at $A,B$ and $C$?

			\item What happened between $D$ and $E$?
		\end{enumerate}
		% TODO Q10
		\item Shown are graphs of the position of two runners, A and B, who run a
			100-m race and finish in a tie.

		\begin{enumerate}
			\item Describe and compare how the runners run the race.

			\item At what time is the distance between the runners the greatest?

			\item At what time do they have the same velocity?
		\end{enumerate}

		% Q11
		\item If a ball is thrown into the air with a velocity of 10 m/s, its height
			(in meters) after $t$ seconds is given by $y = 10t - 4.9t^2$. Find the
			velocity when $t = 2$.

			$$v = \lim \limits _{h \to 0} = \frac{f(t+h) - f(t)}{h}$$
			$$v = \lim \limits _{h \to 0} = \frac{10(t+h) - 4.9(t+h)^2 - (10t - 4.9t^2)}{h}$$
			$$v = \lim \limits _{h \to 0} = \frac{10t + 10h - 4.9t^2 - 9.8th - 4.9h^2 - 10t + 4.9t^2}{h}$$
			$$v = \lim \limits _{h \to 0} = \frac{10h - 9.8th - 4.9h}{h}$$
			$$v = \lim \limits _{h \to 0} = -9.8t - 4.9 h = -9.8t$$

			$$v(t) = -9.8t$$
			$$v(2) = -19.6$$

		% Q12
		\item If an arrow is shot upward on the moon with a velocity of 58 m/s, its height (in meters)
			after $t$ seconds is given by $H = 58t - 0.83t^2$.

		\begin{enumerate}
			\item Find the velocity of the arrow after 1 second.

				$$v = \lim \limits _{h \to 0} \frac{58(t + h) - 0.83(t+h)^2 - (58t - 0.83t^2)}{h}$$

				$$v = \lim \limits _{h \to 0} \frac{58(t+h) - 0.83(t^2+th+h^2)-58t+0.83t^2}{h}$$

				$$v = \lim \limits _{h \to 0} \frac{58t+58h-0.83t^2-0.83th-0.83h^2-58t+0.83t^2}{h}$$

				$$v = \lim \limits _{h \to 0} \frac{58h - 0.83th-0.83h^2}{h}$$

				$$v = \lim \limits _{h \to 0} 58 - 0.83t -0.83h$$

				$$v(t) = 58 - 0.83t$$

				So

				$$v(1) = 58 - 0.83(1) = 57.17 \text{m/s}$$

			\item Find the velocity of the arrow when $t=a$

				$v(a) = 58-0.83a$

			\item When will the arrow hit the moon?

				The velocity of the arrow when its the moon will be the negation of its initial
				velocity so we must solve...

				$$58 - 0.83t = -58$$ 
				$$-0.83t = -58 -58$$
				$$0.83t = 58+58$$
				$$t = \frac{58+58}{0.83}$$
				$$t = \frac{116}{0.83}$$
				$$t = 139.76 \text{ seconds}$$
		\end{enumerate}

		% Q13
		\item The displacement (in meters) of a particle moving in a straight line is given by the equation
			of motion $s = 1/t^2$, where $t$ is measured in seconds. Find the velocity of the particle at
			times $t=a,t=1,t=2$ and $t=3$.

			$$v(t) = \lim \limits _{h \to 0} \frac{ \frac{1}{(t + h)^2} - \frac{1}{t^2} }{h}$$

			$$v(t) = \lim \limits _{h \to 0} \frac{t^2 - (t+h)^2}{ht^2(t+h)^2}$$

			$$v(t) = \lim \limits _{h \to 0} \frac{t^2 - (t^2 + 2th + h^2)}{ht^2(t+h)^2}$$

			$$v(t) = \lim \limits _{h \to 0} \frac{2th+h^2}{ht^2(t+h)^2} = \frac{2t}{t^2t^2}$$

			$$v(t) = \frac{2}{t^3}$$

			So now we can plug in our values...

			$$v(a) = \frac{2}{a^3}$$
			$$v(1) = 2$$
			$$v(2) = \frac{1}{4}$$
			$$v(3) = \frac{2}{27}$$

		% TODO: Q14
		\item The displacement (in meters) of a particle moving in a straight line is given 
			by $s = t^2 - 8t + 18$, where $t$ is measured in seconds.

		\begin{enumerate}
			\item Find the average velocity over each time interval:

			\begin{enumerate}
				\item $[4,3]$

				\item $[3.5,4]$

				\item $[4,5]$

				\item $[4,4.5]$
			\end{enumerate}

			\item Find the instantaneous velocity when $t = 4$.

			\item Draw the graph of $s$ as a function of $t$ and draw the secant lines
				whose slopes are the average velocities in part (a) and the tangent
				line whose slope is the instantaneous velocity in part (b).
		\end{enumerate}

		% TODO: Q15
		\item For the function $g$ whose graph is given, arrange the following numbers in
			increasing order and explain your reasoning:

			\begin{tabular}{ccccc}
				$0$ & $g'(-2)$ & $g'(0)$ & $g'(2)$ & $g'(4)$
			\end{tabular}

		% Q16
		\item Find an equation of the tangent line to the graph of $y = g(x)$ at $x = 5$ if
			$g(5) = -3$ and $g'(5) = 4$.

			The gradient of the graph at $g(5)$ is $4$ as $g'(5) = 4$. So $m = 4$.

			So

			$$y - y_1 = 4(x - x_1)$$

			Because $g(5) = -3$

			$$y - (-3) = 4(x - 5)$$

			$$y + 3 = 4x - 20$$

			$$y = 4x - 23$$

		% Q17
		\item If an equation of the tangent line to the curve $y = f(x)$ at the point where
			$a=2$ is $y = 4x-5$, find $f(2)$ and $f'(2)$

			Because the tangent line is equal to $f(x)$ at 2, $f(2) = 3$. $f'(2)$ is equal
			to the gradient of the tangent at 2 so $f'(2) = 4$.

		% Q18
		\item If the tangent to $y = f(x)$ at $(4,3)$ passes through the point $(0,2)$, find $f(4)$ and
			$f'(4)$.

			$$f(4) = 3$$

			$$m = \frac{3 - 2}{4 - 0} = \frac{1}{4}$$

			So $f'(4) = \frac{1}{4}$

		% TODO: Q19
		\item Sketch the graph of a function $f$ for which $f(0) = 0, f'(0) = 3, f'(1) = 0$, and
			$f'(2) = -1$.

		% TODO: Q20
		\item Sketch the graph of a function $g$ for which
			$g(0) = g(2) = g(4) = 0, g'(1) = g'(3) = 0,$
			$g'(0) = g'(4) = 1, g'(2) = -1, \lim _{x \to \infty} g(x) = \infty,$
			and $\lim _{x \to -\infty} g(x) = -\infty$.

		% Q21
		\item If $f(x) = 3x^2 - x^3,$ find $f'(1)$ and use it to find an equation of the tangent
			line to the curve $y = 3x^2 - x^3$ at the point $(1,2)$.

			$$\lim \limits _{h \to 0} \frac{3(x+h)^2 - (x+h)^3 - [3x^2-x^3]}{h}$$

			$$\lim \limits _{h \to 0} \frac{3(x^2+2xh+h^2)-(x+h)(x^2+2xh+h^2) - [3x^2-x^3]}{h}$$

			$$\lim \limits _{h \to 0} \frac{3(x^2+2xh+h^2)-(x^3+3x^2h+3xh^2+h^3) - [3x^2-x^3]}{h}$$

			$$\lim \limits _{h \to 0} \frac{3x^2+6xh+3h^2-x^3-3x^2h-3xh^2-h^3-3x^2+x^3}{h}$$

			$$\lim \limits _{h \to 0} \frac{6xh+3h^2-3x^2h-3xh^2+h^2}{h}$$

			$$\lim \limits _{h \to 0} 6x + 3h - 3x^2 - 3xh + h^2 = 6x - 3x^2$$

			$$f'(1) = 6(1)-3(1)^2 = 6-3 = 3$$

			$$y - 2 = 3(x - 1)$$

			$$y - 2 = 3x - 3$$

			$$y = 3x - 1$$

		% Q22
		\item If $g(x) = 1 - x^3$, find $g'(0)$ and use it to find an equation of the tangent to the 
			curve $y = 1 - x^3$ at the point $(0,1)$.

		$g(x) = 1 - x^3$ and we need to find $g'(0)$

		$$g'(0) = \lim \limits _{h \to 0} \frac{g(0+h) - g(0)}{h}$$

		$$g'(0) = \lim \limits _{h \to 0} \frac{1 - h^3 - 1}{h}$$

		$$g'(0) = \lim \limits _{h \to 0} h^2 = 0$$

		$$y - 1 = 0(x - 0)$$

		$$y = 1$$

		% TODO: Q23
		\item 
		\begin{enumerate}
			\item If $F(x) = 5x/(1 + x^2)$, find $F'(2)$ and use it to find and equation of the tangent
				line to the curve

				$$y = \frac{5x}{1 + x^2}$$

				at the point $(2,2)$.

			\item Illustrate part (a) by graphing the curve and the tangent line on the same screen.
		\end{enumerate}

		% TODO: Q24
		\item
		\begin{enumerate}
			\item If $G(x) = 4x^2 - x^3$, find $G'(a)$ and use it to find equations of the tangent lines
				to the curve $y = 4x^2 - x^3$ at the points $(2,8)$ and $(3,9)$.

			\item Illustrate part (a) by graphing the curve and the tangent lines on the same screen.
		\end{enumerate}

		\item[25-30] Find $f'(a)$

		% Q25
		\item $f(x) = 3x^2 - 4x + 1$
			
			$$f'(a) = \lim \limits _{h \to 0} \frac{f(a+h) - f(a)}{h}$$

			$$f'(a) = \lim \limits _{h \to 0} \frac{3(a+h)^2 - 4(a+h) + 1 - (3a^2 - 4a + 1)}{h}$$

			$$f'(a) = \lim \limits _{h \to 0} \frac{3(a^2+2ah+h^2) - 4a - 4h + 1 - 3a^2 + 4a - 1}{h}$$

			$$f'(a) = \lim \limits _{h \to 0} \frac{3a^2 + 6ah + 3h^2 - 4a - 4h + 1 - 3a^2 + 4a - 1}{h}$$

			$$f'(a) = \lim \limits _{h \to 0} \frac{6ah + 3h^2 - 4h}{h}$$

			$$f'(a) = \lim \limits _{h \to 0} 6a + 3h - 4$$

			$$f'(a) = 6a - 4$$

		% Q26
		\item $f(t) = t^4 - 5t$

			$$f'(a) = \lim \limits _{h \to 0} \frac{(a+h)^4 - 5(a+h) - (a^4 - 5a)}{h}$$

			$$f'(a) = \lim \limits _{h \to 0} \frac{a^4+4a^3h+6a^2h^2+4ah^3+h^4-5a-5h-a^4+5a}{h}$$

			$$f'(a) = \lim \limits _{h \to 0} \frac{4a^3h + 6a^2h^2 + 4ah^3 + h^4 - 5h}{h}$$

			$$f'(a) = \lim \limits _{h \to 0} 4a^3 + 6a^2h + 4ah^2 + h^3 - 5 = 4a^3 - 5$$

		% Q27
		\item $f(t) = \frac{2t+1}{t+3}$

			$$f'(a) = \lim \limits _{h \to 0} \frac{ \frac{2(a+h)+1}{(a+h)+3} - \frac{2a+1}{a+3}}{h}$$

			$$f'(a) = \lim \limits _{h \to 0} \frac{ \frac{2a + 2h + 1}{a + h + 3} - \frac{2a+1}{a+3} }{h}$$

			$$f'(a) = \lim \limits _{h \to 0} \frac{(2a+2h+1)(a+3) - (a+h+3)(2a+1)}{(a+h+3)(a+3)h}$$

			$$f'(a) = \lim \limits _{h \to 0} \frac{2a^2+2ah+a+6a+6h+3-2a^2-2ah-6a-a-h-3}{h(a+h+3)(a+3)}$$

			$$f'(a) = \lim \limits _{h \to 0} \frac{6h-h}{h(a+h+3)(a+3)}$$

			$$f'(a) = \lim \limits _{h \to 0} \frac{5}{(a+h+3)(a+3)} = \frac{5}{(a+3)^2}$$

		% Q28
		\item $f(x) = x^{-2}$

			$$f'(a) = \lim \limits _{h \to 0} \frac{(a+h)^{-2} - a^{-2}}{h}$$

			$$f'(a) = \lim \limits _{h \to 0} \frac{ \frac{1}{(a+h)^2} - \frac{1}{a^2} }{h}$$

			$$f'(a) = \lim \limits _{h \to 0} \frac{ a^2 - (a+h)^2 }{ha^2(a+h)^2}$$

			$$f'(a) = \lim \limits _{h \to 0} \frac{a^2 - (a^2+2ah+h^2)}{ha^2(a+h)^2}$$

			$$f'(a) = \lim \limits _{h \to 0} \frac{-2ah-h^2}{ha^2(a+h)^2}$$

			$$f'(a) = \lim \limits _{h \to 0} \frac{-2a-h}{a^2(a+h)^2} = - \frac{2a}{a^4} = - \frac{2}{a^3}$$			

		% Q29
		\item $f(x) = \sqrt{1-2x}$

			$$f'(a) = \lim \limits _{h \to 0} \frac{\sqrt{1-2(a+h)} - \sqrt{1-2a}}{h}$$

			$$f'(a) = \lim \limits _{h \to 0} \frac{\sqrt{1-2a-2h} - \sqrt{1-2a}}{h}$$

			We multiply this by $\frac{ \sqrt{1-2a-2h} + \sqrt{1-2a} }{ \sqrt{1-2a-2h} + \sqrt{1-2a}}$

			$$f'(a) = \lim \limits _{h \to 0} \frac{(1-2a-2h) - (1-2a)}{h(\sqrt{1-2a-2h} + \sqrt{1-2a}}$$

			$$f'(a) = \lim \limits _{h \to 0} \frac{-2h}{h(\sqrt{1-2a-2h} + \sqrt{1-2a}}$$

			$$f'(a) = \lim \limits _{h \to 0} \frac{-2}{\sqrt{1-2a-2h} + \sqrt{1-2a}}$$

			$$f'(a) = - \frac{1}{\sqrt{1-2a}}$$
	\end{enumerate}

\end{document}
