\documentclass{article}

\renewcommand{\thesection}{}

\usepackage{amsmath}
\usepackage{gensymb}

\begin{document}

	\section{2.4 Exercises}

	\begin{enumerate}
		\item Find the derivative of $f(x) = (1+2x^2)(x-x^2)$ in two
			ways: by using the Product Rule and by performing the
			multiplication first. Do your answers agree?

			The product rule is $\frac{dy}{dx} fg = (\frac{dy}{dx}f)g + (\frac{dy}{dx}g)f$

			$$f = (1 + 2x^2)$$
			$$\frac{dy}{dx}f = 4x$$
			$$g = x - x^2$$
			$$\frac{dy}{dx} = 1 - 2x$$

			Calculation using the product rule:

			$$\frac{dy}{dx} = (4x)(x-x^2) + (1-2x)(1+2x^2)$$
			$$ = 4x^2 - 4x^3 + [1 + 2x^2 - 2x - 4x^3]$$

			$$ = 4x^2 - 8x^3 + 1 + 2x^2 - 2x$$
			$$ = -8x^3 + 6x^2 - 2x + 1$$

			Calculation by multiplying first:

			$$(1+2x^2)(x-x^2)$$
			$$ = x - x^2 + 2x^3 - 2x^4$$

			$$ f'(x) = 1 - 2x + 6x^2 - 8x^3$$
	\end{enumerate}
\end{document}
