\documentclass{article}

\renewcommand{\thesection}{}

\usepackage{amsmath}

\begin{document}

	\section{2.2 Exercises}

	\begin{enumerate}

		\item[1-2] Use the given graph to estimate the value of each derivative.
			Then sketch the graph of $f'$.

		% TODO: Q1
		\item
		\begin{enumerate}
			\item $f'(-3)$

			\item $f'(-2)$

			\item $f'(0)$

			\item $f'(1)$

			\item $f'(2)$

			\item $f'(3)$
		\end{enumerate}

		% TODO: Q2
		\item
		\begin{enumerate}
			\item $f'(0)$

			\item $f'(1)$

			\item $f'(2)$

			\item $f'(3)$

			\item $f'(4)$

			\item $f'(5)$
		\end{enumerate}

		% TODO: Q3
		\item Match the graph of each function in (a)-(d) with the graph
			of its derivative in I-IV. Give reasons for your choices.

		\item[4-11] Trace or copy the graph of the given function $f$. (Assume
				that the axes have equal scales.) Then use the method
				of Example 1 to sketch the graph of $f'$ below it.

		% TODO: Q4
		\item

		% TODO: Q5
		\item

		% TODO: Q6
		\item

		% TODO: Q7
		\item

		% TODO: Q8
		\item

		% TODO: Q9
		\item

		% TODO: Q10
		\item

		% TODO: Q11
		\item

		% TODO: Q12
		\item Shown is the graph of the population function $P(t)$ for yeast cells
			in a laboratory culture. Use the method of Example 1 to graph the
			derivative $P'(t)$. What does the graph of $P'$ tell us about the
			yeast population?

		% TODO: Q13
		\item A rechargeable battery is plugged into a charger. The graph shows $C(t)$,
			the percentage of full capacity that the battery reaches as a function
			of time $t$ elapsed (in hours).

		\begin{enumerate}
			\item What is the meaning of the derivative $C'(t)$?

			\item Sketch the graph of $C'(t)$. What does the graph tell you?
		\end{enumerate}

		% TODO: Q14
		\item The graph (from the US Department of Energy) shows how driving speed affects
			gas mileage. Fuel economy $F$ is measured in miles per gallon and speed $v$
			is measured miles per hour.

		\begin{enumerate}
			\item What is the meaning of the derivative $F'(v)$?

			\item Sketch the graph of $F'(v)$.

			\item At what speed should you drive if you want to save on gas?
		\end{enumerate}

		% TODO: Q15
		\item The graph shows how the average age of first marriage of Japanese men in
			the last half of the 20th century. Sketch the graph of the derivative function
			$M'(t)$. During which years was the derivative negative?

		% TODO: Q16
		\item Make a careful sketch of the graph of the sine function and below it sketch
			the graph of its derivative in the same manner as in Exercises 4-11. Can you
			guess what the derivative of the sine function is from its graph.

		% TODO: Q17
		\item Let $f(x) = x^2$

		\begin{enumerate}
			\item Estimate the values of $f'(0), f'(\frac{1}{2}), f'(1).$ and $f'(2)$ by
			using a graphing device to zoom in on the graph of $f$.

			\item Use symmetry to deduce the values of $f'(-\frac{1}{2}), f'(1),$ and
				$f'(-2)$.

			\item Use the results from parts (a) and (b) to guess a formula for $f'(x)$.
		\end{enumerate}

		% TODO: Q18
		\item Let $f(x) = x^3$

		\begin{enumerate}
			\item Estimate the values of $f'(0), f'(\frac{1}{2}), f'(1), f'(2),$ and
			$f'(3)$ by using a graphing device to zoom in on the graph of $f$.

			\item Use symmetry to deduce the values of $f'(-\frac{1}{2}), f'(-1), f'(-2),$
				and $f'(-3)$.

			\item Use the values from parts (a) and (b) to graph $f'$.

			\item Use the definition of a derivative to prove your guess in part (d) is correct.
		\end{enumerate}

		\item[19-27] Find the derivative of the function using the definition of derivative. State the
				domain of the function and the domain of its derivative.

		% Q19
		\item $f(x) = \frac{1}{2}x - \frac{1}{3}$

			$$f'(x) = \lim \limits _{h \to 0} \frac{ (\frac{1}{2}(x+h) - \frac{1}{3}) - (\frac{1}{2}x + \frac{1}{3}) }{h}$$

			$$f'(x) = \lim \limits _{h \to 0} \frac{ \frac{1}{2}(x+h) - \frac{1}{2}x }{h}$$

			$$f'(x) = \lim \limits _{h \to 0} \frac{ \frac{1}{2}x + \frac{1}{2}h - \frac{1}{2}x}{h}$$

			$$f'(x) = \lim \limits _{h \to 0} \frac{ \frac{1}{2}h }{h}$$

			$$f'(x) = \lim \limits _{h \to 0} \frac{1}{2} = \frac{1}{2}$$

			The domain of $f(x)$ is $(-\infty, \infty)$. The domain of $f'(x)$ is $(-\infty, \infty)$.

		% Q20
		\item $f(x) = 1.5x^2 - x + 3.7$

			$$f'(x) = \lim \limits _{h \to 0} \frac{(1.5(x+h)^2 - (x+h) + 3.7) - (1.5x^2 - x + 3.7)}{h}$$

			$$f'(x) = \lim \limits _{h \to 0} \frac{1.5(x^2 + 2xh + h^2)-x-h+3.7 - 1.5x^2 + x - 3.7}{h}$$

			$$f'(x) = \lim \limits _{h \to 0} \frac{1.5x^2 + 3xh + 1.5h^2 - x - h + 3.7 - 1.5x^2 - x + 3.7}{h}$$

			$$f'(x) = \lim \limits _{h \to 0} \frac{3xh + 1.5h^2 - h}{h}$$

			$$f'(x) = \lim \limits _{h \to 0} 3x + 1.5h - 1 = 3x - 1$$

			The domain of $f(x)$ is $(-\infty, \infty)$. The domain of $f'(x)$ is $(-\infty, \infty)$.

		% Q21
		\item $f(x) = x^3 - 3x + 5$

			$$f'(x) = \lim \limits _{h \to 0} \frac{(x+h)^3 - 3(x+h) + 5 - (x^3-3x+5)}{h}$$

			$$f'(x) = \lim \limits _{h \to 0} \frac{x^3 + 3x^2h + 3xh^2 + h^3 - 3x - 3h + 5 - x^3 + 3x - 5}{h}$$

			$$f'(x) = \lim \limits _{h \to 0} \frac{3x^2h +3xh^2 + h^3 - 3h}{h}$$

			$$f'(x) = \lim \limits _{h \to 0} 3x^2 + 3xh + h^2 - 3 = 3x^2 - 3$$

			The domain of $f(x)$ is $(-\infty, \infty)$. The domain of $f'(x)$ is $(-\infty, \infty)$.

		% Q22
		\item $f(x) = x + \sqrt{x}$

			$$f'(x) = \lim \limits _{h \to 0} \frac{ [(x+h) + \sqrt{x+h}] - (x + \sqrt{x})}{h}$$

			$$f'(x) = \lim \limits _{h \to 0} \frac{x + h + \sqrt{x+h} - x - \sqrt{x}}{h}$$

			$$f'(x) = \lim \limits _{h \to 0} \frac{\sqrt{x+h} - \sqrt{x} + h}{h}$$

			$$f'(x) = \lim \limits _{h \to 0} \frac{\sqrt{x+h} - \sqrt{x}}{h} + 1$$

			$$f'(x) = \lim \limits _{h \to 0} \frac{x + h - x}{h(\sqrt{x+h} + \sqrt{x}} + 1$$

			$$f'(x) = \lim \limits _{h \to 0} \frac{h}{h(\sqrt{x+h} + \sqrt{x}} + 1$$

			$$f'(x) \lim \limits _{h \to 0} \frac{1}{\sqrt{x+h} + \sqrt{x}} + 1$$

			$$f'(x) = \frac{1}{2\sqrt{x}} + 1$$

			The domain of $f(x)$ is $[0, \infty)$. The domain of $f'(x)$ is $(0, \infty)$.

		% Q23
		\item $g(x) = \sqrt{9-x}$

			$$f'(x) = \lim \limits _{h \to 0} \frac{\sqrt{9-(x+h)} - \sqrt{9-x}}{h}$$

			$$f'(x) = \lim \limits _{h \to 0} \frac{9-(x+h)-(9-x)}{h(\sqrt{9-(x+h)}+\sqrt{9-x})}$$

			$$f'(x) = \lim \limits _{h \to 0} \frac{h}{h(\sqrt{9-(x+h)}+\sqrt{9-x}}$$

			$$f'(x) = \lim \limits _{h \to 0} \frac{1}{\sqrt{9-(x+h)}-\sqrt{9-x}}$$

			$$f'(x) = \frac{1}{2\sqrt{9-x}}$$

		% Q24
		\item $f(x) = \frac{x^2 - 1}{2x - 3}$

			$$f'(x) = \lim \limits _{h \to 0} \frac{\frac{(x+h)^2-1}{2(x+h)-3} - \frac{x^2-1}{2x-3}}{h}$$

			$$f'(x) = \lim \limits _{h \to 0} \frac{[(x+h)^2-1](2x-3) - [2(x+h)-3](x^2-1)}{h[2(x+h)-3](2x-3)}$$

			$$f'(x) = \lim \limits _{h \to 0} \frac{(x^2+2xh+h^2-1)(2x-3)-(2x+2h-3)(x^2-1)}{h}$$

			$$f'(x) = \lim \limits _{h \to 0} \frac{(2x^2+4x^2h+2xh^2-2x-3x^2-6xh-3h^2+3-(2x^3-2x^2h-3x^2-2x-2h+3)}{h}$$

			$$f'(x) = \lim \limits _{h \to 0} \frac{2x^2h+2xh^2-6xh-3h^2+2h}{h[2(x+h)-3](2x-3)}$$

			$$f'(x) = \lim \limits _{h \to 0} \frac{2x^2+2xh-6x-3h+2}{[2(x+h)-3](2x-3)}$$

			$$f'(x) = \frac{2x^2-6x+2}{(2x-3)^2}$$

		% Q25
		\item $G(t) = \frac{4t}{t+1}$

			$$G'(t) = \lim \limits _{h \to 0} \frac{\frac{4(t+h)}{(t+h)+1} - \frac{4t}{t+1}}{h}$$

			$$G'(t) = \lim \limits _{h \to 0} \frac{[4(t+h)](t+1) - 4t[(t+1)+1]}{h[(t+h)+1](t+1)}$$

			$$G'(t) = \lim \limits _{h \to 0} \frac{(4t+4h)(t+1) - (4t^2+4th+4t)}{h(t^2+ht+t+t+h+1)}$$

			$$G'(t) = \lim \limits _{h \to 0} \frac{4t^2+4th+4t+4h-4t^2-4th-4t}{h(t^2+ht+2t+h+1)}$$

			$$G'(t) = \lim \limits _{h \to 0} \frac{4}{t^2+ht+2t+h+1}$$

			$$G'(t) = \frac{4}{t^2+2t+1}$$

			$$G'(t) = \frac{4}{(t+1)^2}$$

		% Q26
		\item $f(x) = x^{3/2}$

			$$f'(x) = \lim \limits _{h \to 0} \frac{(x+h)^{3/2} - x^{3/2}}{h}$$

			$$f'(x) = \lim \limits _{h \to 0} \frac{(x+h)^{3/2} - x^{3/2}{h} \times \frac{(x+h)^{3/2} + x^{3/2}}{(x+h)^{3/2} + x^{3/2}}$$

			$$f'(x) = \lim \limits _{h \to 0} \frac{(x+h)^3 - x^3}{h[(x+h)^{3/2} + x^{3/2}}$$

			$$f'(x) = \lim \limits _{h \to 0} \frac{x^3 - 3x^2h + 3xh^2 + h - x^3}{h[(x+h)^{3/2} + x^{3/2}]}$$	

			$$f'(x) = \lim \limits _{h \to 0} \frac{3x^2 + 3xh}{(x+h)^{3/2} + x^{3/2}}$$

			$$f'(x) = \frac{3x^2}{2x^{3/2}$$

			$$f'(x) = \frac{3\sqrt{x}{2}$$

		% Q27
		\item $f(x) = x^4$

			$$f'(x) = \lim \limits _{h \to 0} \frac{(x+h)^4 - x^4}{h}$$

			$$f'(x) = \lim \limits _{h \to 0} \frac{x^4 + 4x^3h + 6x^2h^2 + 4xh^3 + h^4 - x^4}{h}$$

			$$f'(x) = \lim \limits _{h \to 0} 4x^3 + 6x^2h + 4xh^2 + h^3$$

			$$f'(x) = 4x^3$$
	\end{enumerate}
\end{document}
