\documentclass{article}

\usepackage{amsmath}

\renewcommand{\thesection}{}

\begin{document}

	\section{2.3 Exercises}

	\begin{enumerate}
		\item[1-26] Differentiate the function.

		% Q1
		\item $f(x) = 2^{40}$

			Because this is a constant function

			$$\frac{d}{dx} 2^{40} = 0$$

		% Q2
		\item $f(x) = \sqrt{30}$

			Because this is a constant function

			$$\frac{d}{dx} \sqrt{30} = 0$$

		% Q3
		\item $f(t) = 3 - \frac{2}{3}t$

			$$f'(t) = \frac{d}{dt}3 - \frac{d}{dt} (\frac{2}{3}t)$$

			$$f'(t) = -\frac{2}{3} [\frac{d}{dt} t]$$

			Because $\frac{d}{dt} t = 1$

			$$f'(t) = -\frac{2}{3}$$

		% Q4
		\item $F(x) = \frac{3}{4}x^8$

			$$F'(x) = \frac{3}{4} [\frac{d}{dx} x^8]$$

			Because $\frac{d}{dx} x^8 = 8x^7$

			$$F'(x) = \frac{3}{4} (8x^7) = 6x^7$$

		% Q5
		\item $f(x) = x^3 - 4x + 6$

			$$f'(x) = \frac{d}{dx} x^3 - \frac{d}{dx} 4x + \frac{d}{dx} 6$$

			$$f'(x) = 3x^2 - 4$$	

		% Q6
		\item $f(t) = \frac{1}{2}t^6 - 3t^4 + t$

			$$f'(t) = \frac{d}{dt} [\frac{1}{2}t^6] - \frac{d}{dt} 3t^4 + \frac{d}{dt} t$$

			$$f'(t) = \frac{1}{2} [\frac{d}{dt} t^6] - 3[\frac{d}{dt} t^4] + 1$$

			$$f'(t) = \frac{1}{2} (6t^5) - 3(4t^3) + 1$$

			$$f'(t) = 3t^5 - 12t^3 + 1$$

		% Q7
		\item $f(x) = 3x^2 - 2\cos x$

			$$f'(x) = \frac{d}{dx} 3x^2 - \frac{d}{dx} 2\cos x$$

			$$f'(x) = 3 [\frac{d}{dx} x^2] - 2 [\frac{d}{dx} \cos x$$

			$$f'(x) = 3 (2x) - 2 (-\sin x)$$

			$$f'(x) = 6x + 2\sin x$$

		% Q8
		\item $y = \sin t + \pi \cos t$

			$$\frac{dy}{dt} = \frac{d}{dt} (\sin x) + \frac{d}{dt} (\pi \cos t)$$

			$$\frac{dy}{dt} = \cos x + \pi [\frac{d}{dt} \cos t]$$

			$$\frac{dy}{dt} = \cos x + \pi (- \sin t)$$

			$$\frac{dy}{dt} = \cos x - \pi \sin t$$

		% Q9
		\item $g(x) = x^2(1-2x)$

			Although we could solve this using the product rule, lets expand the brackets.

			$$g(x) = x^2 - 2x^3$$

			$$g'(x)  = \frac{d}{dx} x^2 - \frac{d}{dx} [2x^3]$$

			$$g'(x)  = 2x - 2 [\frac{d}{dx} x^3]$$

			$$g'(x) = 2x - 2 (3x^2)$$

			$$g'(x) = 2x - 6x^2$$

		% Q10
		\item $h(x) = (x-2)(2x + 3)$

			Lets expand this out into a polynomial that we can differentiate with the power rule.

			$$h(x) = 2x^2 + 3x - 4x - 6$$

			$$h(x) = 2x^2 - x - 6$$

			$$h'(x) = \frac{d}{dx} (2x^2) - \frac{d}{dx} x - \frac{d}{dx} 6$$

			$$h'(x) = 2 [ \frac{d}{dx}x^2] - 1$$

			$$h'(x) = 2(2x) - 1$$

			$$h'(x) = 4x - 1$$

		% Q11
		\item $y = x^{-2/5}$

			$$\frac{dy}{dx} = \frac{d}{dx} x^{-2/5}$$

			$$\frac{dy}{dx} = -\frac{2 x^{-7/5}}{5}$$

		% Q12
		\item $B(y) = cy^{-6}$

			Here we are treating $c$ as a constant

			$$B'(y) = \frac{d}{dy} (cy^{-6})$$

			$$B'(y) = c [\frac{d}{dy} y^{-6}$$

			$$B'(y) = c(-6y^{-7})$$

			$$B'(y) = -6cy^{-7}$$

		% Q13
		\item $A(s) = - \frac{12}{s^{5}}$

			We can express this as 

			$$A(s) = - 12s^{-5}$$

			$$A'(s) = \frac{d}{ds} [-12s^{-5}]$$

			$$A'(s) = -12 [\frac{d}{ds} s^{-5}]$$

			$$A'(s) = -12 (-5 s^{-6})$$

			$$A'(s) = 60 s^{-6}$$

		% Q14
		\item $y = x^{5/3} - x^{2/3}$

			$$\frac{dy}{dx} = \frac{d}{dx} x^{5/3} - \frac{d}{dx} x^{2/3}$$

			$$\frac{dy}{dx} = \frac{5 x^{2/3}}{3} - \frac{2}{3x^{1/3}}$$

		% Q15
		\item $R(a) = (3a + 1)^2$

			$$R(a) = 6a^2 + 6a + 1$$

			$$R'(a) = \frac{d}{da} [6a^2] + \frac{d}{da} [6a] + \frac{d}{da} 1$$

			$$R'(a) = 6 [\frac{d}{da} a^2] + 6 [\frac{d}{da} a]$$

			$$R'(a) = 6 (2a) + 6 (1) + 1$$

			$$R'(a) = 12a + 6$$	

		% Q16
		\item $y = \sqrt{x}(x - 1)$

			$$y = x \sqrt{x} - \sqrt{x}$$

			$$y = x \dot x^{1/2} - \sqrt{x}$$

			$$y = x^{3/2} - x^{1/2}$$

			$$\frac{dy}{dx} = \frac{d}{dx} x^{3/2} - \frac{d}{dx} x^{1/2}$$

			$$\frac{dy}{dx} = \frac{3\sqrt{x}}{2} - \frac{1}{2\sqrt{x}}$$

		% Q17
		\item $S(p) = \sqrt{p} - p$

			$$S'(p) = \frac{d}{dp} p^{1/2} - \frac{d}{dp} p$$

			$$S'(p) = \frac{1}{2} p^{-1/2} - 1$$

		% Q18
		\item $S(R) = 4 \pi R^2$

			$$S'(R) = \frac{d}{dR} 4 \pi R^2$$

			$$S'(R) = 4 \pi [\frac{d}{dR} R^2$$

			$$S'(R) = 4 \pi (2R)$$

			$$S'(R) = 8 \pi R$$

		% Q19
		\item $y = \frac{x^2 + 4x + 3}{\sqrt{x}}$

			$$y = (x^2 + 4x + 3)(x^{-1/2})$$

			$$y = x^{3/2} + 4x^{1/2} + 3x^{-1/2}$$

			$$\frac{dy}{dx} = \frac{d}{dx} x^{3/2} + \frac{d}{dx} 4x^{1/2} + \frac{d}{dx} x^{-1/2}$$

			$$\frac{dy}{dx} = \frac{3x^{1/2}}{2} + 4 [\frac{d}{dx} x^{1/2}] - \frac{1}{2x^{3/2}}$$

			$$\frac{dy}{dx} = \frac{3x^{1/2}}{2} + \frac{2}{x^{1/2}} - \frac{1}{2x^{3/2}}$$

		% Q20
		\item $g(u) = \sqrt{2}u + \sqrt{3u}$

			$$g'(u) = \frac{d}{du} \sqrt{2}u + \frac{d}{du} \sqrt{3u}$$

			We can work out $frac{d}{du} \sqrt{3u}$ using the chain rule or from the 
			definition of a derivative.

			$$\frac{d}{du} \sqrt{3u} = \lim \limits _{h \to 0} \frac{\sqrt{3(u+h)} - \sqrt{3u}}{h}$$

			We multiply this by $\frac{\sqrt{3(u+h)} + \sqrt{3u}}{\sqrt{3(u+h) + \sqrt{3u}}}$

			$$\frac{d}{du} \sqrt{3u} = \lim \limits _{h \to 0} \frac{3(u+h) - 3u}{h(\sqrt{3(u+h)} + \sqrt{3u}}$$

			$$\frac{d}{du} \sqrt{3u} = \lim \limits _{h \to 0} \frac{3h}{h(\sqrt{3(u+h)} + \sqrt{3u}}$$
			
			$$\frac{d}{du} \sqrt{3u} = \lim \limits _{h \to 0} \frac{3}{\sqrt{3(u+h)} + \sqrt{3u}}$$

			$$\frac{d}{du} \sqrt{3u} = \frac{3}{2\sqrt{3u}}$$

			We can use this result to solve the original derivative.

			$$g'(u) = \sqrt{2} \frac{d}{du} u + \frac{3}{2\sqrt{3u}}$$
			
			$$g'(u) = \sqrt{2} + \frac{3}{2\sqrt{3u}}$$

		% Q21
		\item $v = t^2 - \frac{1}{\sqrt[4]{t^3}}$

			$$\frac{dv}{dt} = \frac{d}{dt} t^2 - \frac{d}{dt} \frac{1}{\sqrt[4]{t^3}}$$

			$$\frac{dv}{dt} = 2t - \frac{d}{dt} t^{-3/4}$$

			$$\frac{dv}{dt} = 2t + \frac{3}{4} t^{-7/4}$$

		% Q22
		\item $y = \frac{x^2 - 2\sqrt{x}}{x}$

			$$y = \frac{x^2}{x} - \frac{2\sqrt{x}}{x}$$

			$$y = x - 2x^{-1/2}$$

			$$\frac{dy}{dx} = \frac{d}{dx} x - \frac{d}{dx} 2x^{-1/2}$$

			$$\frac{dy}{dx} = 1 + x^{-3/2}$$

		% Q23
		\item $z = \frac{A}{y^{10}} + B \cos y$

			$$\frac{dz}{dy} = \frac{d}{dy} Ay^{-10} + \frac{d}{dy} B \cos y$$

			$$\frac{dz}{dy} = A [\frac{d}{dy} y^{-10}] + B [\frac{d}{dy} \cos y$$

			$$\frac{dz}{dy} = A (-10y^{-11}) + B [ - \sin y]$$

			$$\frac{dz}{dy} = -10Ay^{-11} - B\sin y$$

		% Q24
		\item $y = \frac{\sin \theta}{2} + \frac{c}{\theta}$

			$$y = \frac{1}{2} \sin \theta + c \theta^{-1}$$

			$$\frac{dy}{d\theta} = \frac{d}{d\theta} (\frac{1}{2} \sin \theta) + \frac{d}{d\theta} (c \theta^{-1})$$

			$$\frac{dy}{d\theta} = \frac{1}{2} [ \frac{d}{d\theta} \sin \theta ] + c [ \frac{d}{d\theta} \theta^{-1}]$$

			$$\frac{dy}{d\theta} = \frac{1}{2} (\cos \theta) + c (- \theta^{-2})$$

			$$\frac{dy}{d\theta} = \frac{1}{2} \cos \theta - c \theta^{-2}$$

		% Q25
		\item $H(x) = (x + x^{-1})^{3}$

			Lets expand this out

			$$H(x) = x^3 + 3x^2(x^{-1}) + 3x(x^{-1})^{2} + (x^{-1})^{3}$$

			$$H(x) = x^3 + 3x + 3x \dot x^{-2} + x^{-3}$$

			$$H(x) = x^3 + 3x + 3x^{-1} + x^{-3}$$

			$$H'(x) = 3x^2 + 3 - 3x^{-2} - 3x^{-4}$$

		% Q26
		\item $u = \sqrt[3]{t^2} + 2\sqrt{t^3}$

			$$u = t^{2/3} + 2t^{3/2}$$

			$$\frac{du}{dt} = \frac{d}{dt} t^{2/3} + \frac{d}{dt} 2t^{3/2}$$

			$$\frac{du}{dt} = \frac{2}{3} t^{-1/3} + 2[\frac{d}{dt} t^{3/2}]$$

			$$\frac{du}{dt} = \frac{2}{3} t^{-1/3} + \frac{6}{2} t^{1/2}$$
			$$\frac{du}{dt} = \frac{2}{3} t^{-1/3} + 3t^{1/2}$$

		\item[27-28] Find equations of the tangent line and the normal line to
				the curve at the given point.

		% Q27
		\item $y = 6 \cos x, (\pi/3,3)$

			First lets differentiate the equation

			$$y' = - 6 \sin x$$

			$$y'(\pi/3) = - 6 \sin (\pi/3)$$

			$$\sin \frac{\sqrt{3}}{2}$$

			$$y'(\pi/3) = - 6 \frac{\sqrt{3}}{2} = - 3 \sqrt{3}$$

			We can then use the point - slope equation to get the tangent line.

			$$y - 3 = - 3 \sqrt{3} ( x - \frac{\pi}{3} )$$

			$$y - 3= - 3x\sqrt{3} + \pi \sqrt{3}$$

			$$y = - 3x\sqrt{3} + \pi \sqrt{3} + 3$$

			To get the equation for the normal we must find the gradient of the perpendicular

			$$ = \frac{1}{3\sqrt{3}}$$

			And use the point - slope again.

			$$y - 3 = \frac{1}{3\sqrt{3}} (x - \frac{\pi}{3})$$

			$$y - 3 = \frac{x}{3\sqrt{3}} - \frac{\pi}{\sqrt{3}$$

			$$ = \frac{x}{3\sqrt{3}} - \frac{\pi}{\sqrt{3}} + 3$$

		% Q28
		\item $y = (1 + 2x)^2, (1,9)$

			First lets expand the equation

			$$y = 4x^2 + 4x + 1$$

			Now lets differentiate...

			$$y' = 8x + 4$$

			The gradient of the curve at 1 is...

			$$y'(1) = 8(1) + 4 = 12$$

			Using the point - slope method we can determine an equation for the tangent

			$$y - 9 = 12(x -1)$$

			$$y - 9 = 12x - 12$$

			$$y = 12x - 12 + 9 = 12x - 3$$

			The normal is perpendicular to the tangent

			$$m = -\frac{1}{12}$$

			Using the point - slope method we can determine an equation for the normal

			$$y - 9 = -\frac{1}{12}(x - 1)$$

			$$y - 9 = -\frac{1}{12}x + \frac{1}{12}$$

			$$y = -\frac{x}{12} + 9 + \frac{1}{12}$$

		\item[31-34] Find the first and sercond derivatives of the function.

		% Q31
		\item $f(x) = x^4 - 3x^3 + 16x$

			$$f'(x) = \frac{d}{dx} x^4 - \frac{d}{dx} 3x^3 + \frac{d}{dx} 16x$$

			$$f'(x) = 4x^3 - 3[\frac{d}{dx} x^3] + 16 [\frac{d}{dx} x]$$

			$$f'(x) = 4x^3 - 3[3x^2] + 16[1]$$

			$$f'(x) = 4x^3 - 9x^2 + 16$$

			$$f''(x) = \frac{d}{dx} 4x^3 - \frac{d}{dx} 9x^2 + \frac{d}{dx} 16$$

			$$f''(x) = 4[\frac{d}{dx} x^3] - 9[\frac{d}{dx} x^2]$$

			$$f''(x) = 4[3x^2] - 9[2x]$$

			$$f''(x) = 12x^2 - 18x$$

		% Q32
		\item $G(r) = \sqrt{r} + \sqrt[3]{r}$

			$$G(r) = r^{1/2} + r^{1/3}$$

			$$G'(r) = \frac{d}[dx} r^{1/2} + \frac{d}{dx} r^{1/3}$$

			$$G'(r) = \frac{1}{2} r^{-1/2} + \frac{1}{3} r^{-2/3}$$

			$$G''(r) = - \frac{1}{4} r^{-3/2} - \frac{2}{9} r^{-5/3}$$

		% Q33
		\item $g(t) = 2\cos t - 3 \sin t$

			$$g'(t) = \frac{d}{dt} 2\cos t - \frac{d}{dt} 3 \sin t$$

			$$g'(t) = 2[\frac{d}{dt} \cos t] - 3 [\frac{d}{dt} \sin t]$$

			$$g'(t) = 2[-\sin t] - 3[\cos t]$$

			$$g'(t) = 3 \cos t - 2 \sin t$$

			$$g''(t) = - 3 \sin t - 2 \cos t$$

		% Q34
		\item $h(t) = \sqrt{t} + 5 \sin t$

			$$h(t) = t^{1/2} + 5\sin t$$

			$$h'(t) = \frac{1}{2} t^{-1/2} + 5 \cos t$$

			$$h''(t) = -\frac{1}{4} t^{-3/2} - 5 \sin t$$

		% Q35
		\item Find $\frac{d^{99}}{dx^{99}} (\sin x)$

			Lets do the first few derivations

			$$\frac{d}{dx} (\sin x) = \cos x$$

			$$\frac{d^{2}}{dx^{2}} (\sin x) = -\sin x$$

			$$\frac{d^{3}}{dx^{3}} (\sin x) = -\cos x$$

			$$\frac{d^{4}}{dx^{4}} (\sin x) = \sin x$$

			$$\frac{d^{5}}{dx^{5}} (\sin x) = \cos x$$

			$$\frac{d^{6}}{dx^{6}} (\sin x) = -\sin x$$

			$$\frac{d^{7}}{dx^{7}} (\sin x) = -\cos x$$

			$$\frac{d^{8}}{dx^{8}} (\sin x) = \sin x$$

			Now, the factors of 99 are 3, 3 and 11.

			We can see above that derivatives that are multiples
			of 3 are $-\sin x$

			So $$\frac{d^{99}}{dx^{99}} (\sin x) = -\sin x$$

		% Q36
		\item Find the $n$th derivative of each function by calculating the
			first few derivatives and observing the pattern that occurs.

		\begin{enumerate}
			\item $f(x) = x^{n}$

			We will assume here that $n$ is a positive integer, and for clarity find
			the $r$th derivative

			$$f(x) = x^{n}$$

			$$f'(x) = nx^{n-1}$$

			$$f'(x) = n(n-1)x^{n-2}$$

			$$f'(x) = n(n-1)(n-2)x^{n-3}$$

			So we can see the exponent will be $n-r$ while the
			coefficient will be $n! - (n-r)!$

			$$[n! - (n-r)!]x^{n-r}$$

			\item $f(x) = \frac{1}{x}$

			If we calculate the first few derivatives

			$$f(x) = \frac{1}{x}$$

			$$f'(x) = \frac{-1}{x^2}$$

			$$f''(x) = \frac{(-1)(-2)}{x^{3}}$$

			$$f'''(x) = \frac{(-1)(-2)(-3)}{x^{4}}$$

			So the $n$th derivative is

			
			$$\frac{(-1)(-2)...(-n)}{x^{n+1}$$
		\end{enumerate}

		% Q37
		\item For what values of $x$ does the graph of $f(x) = x + 2\sin x$
			have a horizontal tangent?

			To find the horizontal tangents we need to find the points at
			the derivatives $f'(x) = 0$

			$$f'(x) = 1 + 2\cos x$$

			$$1 + 2\cos x = 0$$

			$$2 \cos x = -1$$

			$$\cos x = - \frac{1}{2}$$

			On the unit circle $\cos (\frac{2\pi}{3}) = -\frac{1}{2}$ and
			$\cos (\frac{4\pi}{3}) = -\frac{1}{2}$

			So the horizontal tangents are at...

			$$\frac{2\pi}{3} + k\pi, \frac{4\pi}{3} + k\pi$$ where $k$ is
			an integer.

		% Q38
		\item For what values of $x$ does the graph of 
			$f(x) = x^3 + 3x^2 + x + 4$ have a horizontal tangent?

			First we need to find the derivative.

			$$f'(x) = 3x^2 + 6x + 1$$

			And find the roots of the equation.

			$$3x^2 + 6x + 1 = 0$$

			Which we can do by completing the square.

			$$3x^2 + 6x = -1$$

			$$x^2 + 2x = -\frac{1}{3}$$

			$$x^2 + 2x + 1 = 1 - \frac{1}{3}$$

			$$(x+1)^2 = 1 - \frac{1}{3}$$

			$$(x+1)^2 = \frac{2}{3}$$

			$$x + 1 = \pm \sqrt{\frac{2}{3}}$$

			$$x = -1 \pm \sqrt{\frac{2}{3}}$$

		% Q39
		\item Show that the curve $y = 6x^3 + 5x - 3$ has no tangent
			line with slope 4.


			$$y = 6x^3 + 5x - 3$$

			$$y' = 18x^2 + 5$$

			$$18x^2 + 5 = 4$$

			$$18x^2 + 1 = 0$$

			We can use the quadratic descriminant to show there are no solutions.

			$$b^2 - 4ac$$

			$$0 - 4 (18) (1)$$

			$$-72 < 0$$

		% Q40
		\item Find an equation of the tangent line to the curve $y = x\sqrt{x}$ that
			is parallel to the line $y = 1 + 3x$

			The gradient of the tangent line is 3.

			We need to find the point on the curve where the gradient is 3.

			$$y = x . x^{1/2} = x^{3/2}$$

			$$y' = \frac{3\sqrt{x}}{2}$$

			So we need to solve for $x$...

			$$\frac{3\sqrt{x}}{2} = 3$$

			$$3\sqrt{x} = 6$$

			$$\sqrt{x} = 2$$

			$$x = 4$$

			And we can put this in our original equation to get $y$

			$$y = 4\sqrt{4} = 8$$

			And now use point-slope line equation form to find a parallel tangent

			$$y - 8 = 3(x - 4)$$

			$$y - 8 = 3x - 12$$

			$$y = 3x - 4$$

		% Q41
		\item Find an equation of the normal line to the parabola $y = x^2 - 5x + 4$ that
			is parallel to the line $x - 3y = 5$.

			We are looking for a line parallel to $x - 3y = 5$

			If we rearrange this so that $y$ is on the left we have $y = \frac{1}{3} - \frac{5}{3}$.

			So we are looking for a line with a gradient of $\frac{1}{3}$, the perpendicular will
			have a gradient of $-3$. So to find a normal on the curve that is perpendicular to
			the line we must find a point on the curve where the tangent has a gradient of $-3$.

			If we differentiate the curve we get $y' = 2x - 5$. We want to find the value of $x$
			where $y' = -3$, so

			$$2x - 5 = -3$$

			$$2x = 2$$

			$$x = 1$$

			We must also know the value of $y$ when $x = 1$ so

			$$(1)^2 - 5(1) + 4 = 0$$

			So the normal equation is...

			$$y - 0 = \frac{1}{3}(x - 1)$$

			$$y = \frac{x}{3} - \frac{1}{3}$$

		% TODO Q42

		% Q43
		\item The equation of motion of a particle is $s = t^3 - 3t$, where $s$ is in meters and
			$t$ is in seconds. Find

		\begin{enumerate}
			\item the velocity and acceleration as functions of $t$.

			The velocity is the first derivative so

			$$s' = 3t^2 - 3$$

			The acceleration is the second derivatrive so...

			$$s'' = 6t$$

			\item the acceleration after 2 s

			$$s''(2) = 6(2) = 12 \text{ metres per second per second}$$

			\item the acceleration when the velocity is 0.

				$$3t^2 - 3 = 0$$

				$$3t^2 = 3$$

				$$t^2 = 1$$

				$$t = \pm 1$$

				So if we plug this into the equation of acceleration

				$$6(1) = 6$$
		\end{enumerate}

		% TODO: Q44
		% TODO: Q45
		% TODO: Q46

		% Q47
		\item The position function of a particle is given by $s = t^3 - 4.5t^2 - 7t, t \geq 0$.

			\begin{enumerate}
				\item When does the particle reach a velocity of 5 m/s?

				First we find the derivative...

				$$s' = 3t^2 - 9t -7$$

				And find the value of $t$ when $3t^2 - 9t - 7 = 5$

				$$3t^2 - 9t - 2 = 0$$

				$$t^2 - 3t - \frac{2}{3} = 0$$

				Let's find the value of $t$ by completing the square.

				$$t^2 - 3t = \frac{2}{3}$$

				$$t^2 - 3t + \frac{9}{4} = \frac{2}{3} + \frac{9}{4}$$

				$$(t - \frac{3}{2})^2 = \frac{35}{12}$$

				$$t - \frac{3}{2} = \pm \sqrt{\frac{35}{12}}$$

				$$t = \frac{3}{2} = \pm \sqrt{\frac{35}{12}}$$

				The only positive result is

				$$t = \frac{3}{2} + \sqrt{\frac{35}{12}} = 3.208$$

				\item When is the acceleration 0? What is the significance
					of this value of $t$?

					When we differentiate to get the equation for acceleration
					we get $s'' = 6t$

					Thus the acceleration is 0 when $t = 0$. This is significant
					as it is the initial value of $t$.
			\end{enuemrate}

			% Q48
			\item If a ball is given a push so that it has an initial velocity of 5 m/s
				down a certain inclined plane, then the distance it has rolled down
				after $t$ seconds is $s = 5t + 3t^2$/

			\begin{enumerate}
				\item Find the velocity after 2 s.

				$$s' = 5 + 6t$$

				$$s'(2) = 5 + 6(2) = 17$$

				\item How long does it take for the velocity to reach 35 m/s?

					$$5 + 6t = 35$$

					$$6t = 30$$

					$$t = \frac{30}{6} = 5$$
			\end{enumerate}

			% Q49
			\item If a rock is thrown vertically upward from the surface of Mars with
				velocity 15 m/s, its height after $t$ seconds is $h = 15t - 1.86t^2$.

				\begin{enumerate}
					\item What is the velocity of the rock after 2 s?

						First we have to differentiate the position equation to
						get the velocity equation

						$$h' = 15 - 3.72t$$

						$$h'(2) = 15 - 3.72(2) = 7.56 \text{ m/s }$$

					\item What is the velocity of the rock when its height is 25 m
						on its way up? On its way down?

						We need to find the value of $t$ when $h = 25$.

						$$15t - 1.86t^2 = 25$$

						$$15t - 1.86t^2 - 25 = 0$$

						The solutions to this equation (from an equation solver)
						are $h = 2.353, 5.711$.

						We can find the velocity by plugging these values into the 
						first derivative.

						$$15 - 3.72(2.353) = 6.247 \text{ m/s }$$

						The second value is the velocity on the way down.

						$$15 - 3.72(5.711) = -6.245 \text{ m/s }$$

				\end{enumerate}

		% Q50
		\item If a ball is thrown vertically upward with a velocity of 24.5 m/s, then its height
			after $t$ seconds is $s = 24.5t - 4.9t^2$.

				\begin{enumerate}

					\item What is the maximum height reached by the ball?

						First we differentiate and find the value of $t$ where the
						gradient is 0.

						$$s' = 24.5 - 9.8t$$

						$$24.5 - 9.8t = 0$$

						$$9.8t = 24.5$$

						$$t = \frac{24.5}{9.8} = 2.5$$

						Then we plug that into our original equation

						$$24.5(2.5) - 4.9(2.5)^2 = 30.625$$

					\item What is the velocity of the ball when it is 29.4 m above
						the ground on its way up? On its way down?

						$$24.5t - 4.9t^2 = 29.4$$

						$$4.9t^2 - 24.5t + 29.4 = 0$$

						$$t^2 - 5t + 9 = 0$$

						$$(t-2)(t-3) = 0$$

						Velocity on the balls way up is

						$$24.5 - 9.8(2) = 4.9$$

						Velocity on the way down is

						$$24.5 - 9.8(3) = -4.9$$
				\end{enumerate}
					
	\end{enumerate}	
\end{document}
